src/syntax.mli
@@ -19,6 +19,7 @@ module StringSet : Set.S with type elt = string
 
 val formula_to_string : ?outer:int -> formula -> string
 val term_to_string : term -> string
+val term_free_vars : term -> StringSet.t
 val free_vars : formula -> StringSet.t
 val all_vars : formula -> StringSet.t
 val fresh_name : string -> StringSet.t -> string
